DynamoDbItemEncryptor/src/ConfigToInfo.dfy
@@ -1,0 +1,304 @@
+// Copyright Amazon.com Inc. or its affiliates. All Rights Reserved.
+// SPDX-License-Identifier: Apache-2.0
+
+include "../Model/AwsCryptographyDynamoDbItemEncryptorTypes.dfy"
+include "../../StructuredEncryption/src/SearchInfo.dfy"
+include "Util.dfy"
+include "FakeConfig.dfy"
+
+module SearchConfigToInfo {
+  import opened AwsCryptographyDynamoDbItemEncryptorTypes
+  import opened StandardLibrary
+  import opened Wrappers
+  import opened StandardLibrary.UInt
+  import opened DynamoDbItemEncryptorUtil
+
+  import C = SearchableEncryptionParseConfig
+  import I = SearchableEncryptionInfo
+  import V = VirtualFields
+  import U = StructuredEncryptionUtil
+  import P = StructuredEncryptionPaths
+  import B = BaseBeacon
+  import CB = CompoundBeacon
+  import SE = AwsCryptographyStructuredEncryptionTypes
+  import Prim = AwsCryptographyPrimitivesTypes
+  import Aws.Cryptography.Primitives
+
+  method Convert(outer : DynamoDbItemEncryptorConfig, config : Option<C.SearchConfig>)
+    returns (ret : Result<Option<I.SearchInfo>, Error>)
+    ensures ret.Success? && ret.value.Some? ==>
+      && ret.value.value.ValidState()
+  {
+    if config.None? {
+      return Success(None);
+    } else {
+      :- Need(config.value.writeVersion == 1, E("writeVersion must be '1'."));
+      :- Need(|config.value.versions| == 1, E("search config must be have exactly one version."));
+      var version :- ConvertVersion(outer, config.value.versions[0]);
+      var info := I.SearchInfo(versions := [version], currWrite := 0);
+      var _ :- info.CheckValid().MapFailure(e => AwsCryptographyStructuredEncryption(e));
+      return Success(Some(info));
+    }
+  }
+  
+  function method GetPersistentKey(keyring: AwsCryptographyMaterialProvidersTypes.IKeyring)
+    : Result<U.Bytes, Error>
+  {
+    Success([1,2,3,4,5])
+  }
+
+  method GetBeaconKey(client : Primitives.AtomicPrimitivesClient, key : U.Bytes, name : string)
+    returns (output : Result<U.Bytes, Error>)
+    modifies client.Modifies
+    requires client.ValidState()
+    ensures client.ValidState()
+  {
+    var info :- UTF8.Encode("AWS_DBE_SCAN_BEACON" + name).MapFailure(e => E(e));
+    var foo := client.Hkdf(Prim.HkdfInput(
+      digestAlgorithm := Prim.SHA_512,
+      salt := None,
+      ikm := key,
+      info := info,
+      expectedLength := 64
+    ));
+    return Failure(E(""));
+  }
+
+  method ConvertVersion(outer : DynamoDbItemEncryptorConfig, config : C.BeaconVersion)
+    returns (output : Result<I.BeaconVersion, Error>)
+  {
+    :- Need(config.version == 1, E("Version number in BeaconVersion must be '1'."));
+    :- Need((config.standardBeacons.Some? && 0 < |config.standardBeacons.value|)
+         && (config.compoundBeacons.Some? && 0 < |config.compoundBeacons.value|),
+         E("At least one beacon must be configured."));
+    var maybePrimitives := Primitives.AtomicPrimitives();
+    // TODO var primitives :- maybePrimitives.MapFailure(e => AwsCryptographyPrimitives(e));
+    var primitives :- maybePrimitives.MapFailure(e => E("Bad primitives construction"));
+
+    var virtualFields :- ConvertVirtualFields(outer, config.virtualFields);
+    var key :- GetPersistentKey(config.keyring);
+    var beacons :- ConvertBeacons(outer, key, primitives, virtualFields, config.standardBeacons.UnwrapOr([]), config.compoundBeacons.UnwrapOr([]));
+    return Success(I.BeaconVersion(
+      version := config.version as I.VersionNumber,
+      beacons := beacons,
+      virtualFields := virtualFields
+    ));
+  }
+
+  function method ConvertVirtualFields(outer : DynamoDbItemEncryptorConfig, vf : Option<C.VirtualFieldList>)
+    : Result<I.VirtualFieldMap, Error>
+  {
+    if vf.None? then
+      Success(map[])
+    else
+      AddVirtualFields(vf.value, outer)
+  }
+
+  predicate method IsSigned(outer : DynamoDbItemEncryptorConfig, loc : P.TerminalLocation)
+  {
+    && var name := loc.parts[0].key;
+    && name in outer.attributeActions
+    && outer.attributeActions[name] != SE.DO_NOTHING
+  }
+
+  predicate method IsEncrypted(outer : DynamoDbItemEncryptorConfig, loc : P.TerminalLocation)
+  {
+    && var name := loc.parts[0].key;
+    && name in outer.attributeActions
+    && outer.attributeActions[name] != SE.DO_NOTHING
+  }
+
+  predicate method IsEncryptedV(outer : DynamoDbItemEncryptorConfig, virtualFields : I.VirtualFieldMap, loc : P.TerminalLocation)
+  {
+    var name := loc.parts[0].key;
+    if name in outer.attributeActions then
+      outer.attributeActions[name] != SE.ENCRYPT_AND_SIGN
+    else if name in virtualFields then
+      var vf := virtualFields[name];
+      // A virtual field is encrypted if any part is encrypted
+      vf.examine((t : P.TerminalLocation) => IsEncrypted(outer, t))
+    else
+      false
+  }
+
+  function method CheckExists(outer : DynamoDbItemEncryptorConfig, name : string, context : string)
+    : Result<bool, Error>
+  {
+    if name in outer.attributeActions then
+      Failure(E(name + " not allowed as a " + context + " because it is already a configured attribute."))
+    else if outer.allowedUnauthenticatedAttributes.Some? && name in outer.allowedUnauthenticatedAttributes.value then
+      Failure(E(name + " not allowed as a " + context + " because it is already an allowed unauthenticated attribute."))
+    else if outer.allowedUnauthenticatedAttributePrefix.Some? && outer.allowedUnauthenticatedAttributePrefix.value <= name then
+      Failure(E(name + " not allowed as a " + context + " because it begins with the allowed unauthenticated prefix."))
+    else if U.ReservedPrefix <= name then
+      Failure(E(name + " not allowed as a " + context + " because it begins with the reserved prefix."))
+    else
+      Success(true)
+  }
+
+  function method {:tailrecursion} AddVirtualFields(
+      vf : seq<C.VirtualField>,
+      outer : DynamoDbItemEncryptorConfig,
+      converted : I.VirtualFieldMap := map[])
+    : Result<I.VirtualFieldMap, Error>
+  {
+    if |vf| == 0 then
+      Success(converted)
+    else
+      :- Need(vf[0].name !in converted, E("Duplicate VirtualField name : " + vf[0].name));
+      var _ :- CheckExists(outer, vf[0].name, "VirtualField");
+      var newField :- V.GetVirtualField(vf[0].name, vf[0].config).MapFailure(e => E(e));
+      // need all parts signed
+      :- Need(!newField.examine((t : P.TerminalLocation) => !IsSigned(outer, t)),
+        E("VirtualField " + vf[0].name + " must be defined on signed fields."));
+      AddVirtualFields(vf[1..], outer, converted[vf[0].name := newField])
+  }
+
+  method {:tailrecursion} AddStandardBeacons(
+      beacons : seq<C.StandardBeacon>,
+      outer : DynamoDbItemEncryptorConfig,
+      key : U.Bytes,
+      client: Primitives.AtomicPrimitivesClient,
+      virtualFields : I.VirtualFieldMap,
+      converted : I.BeaconMap := map[])
+    returns (output : Result<I.BeaconMap, Error>)
+    modifies client.Modifies
+    requires client.ValidState()
+    ensures client.ValidState()
+  {
+    if |beacons| == 0 {
+      return Success(converted);
+    }
+    :- Need(beacons[0].name !in converted, E("Duplicate StandardBeacon name : " + beacons[0].name));
+    var _ :- CheckExists(outer, beacons[0].name, "StandardBeacon");
+    var newKey :- GetBeaconKey(client, key, beacons[0].name);
+    var locString := if beacons[0].loc.Some? then beacons[0].loc.value else beacons[0].name;
+    var newBeacon :- B.MakeStandardBeacon(client, beacons[0].name, newKey, beacons[0].length as B.BeaconLength, locString)
+      .MapFailure(e => AwsCryptographyStructuredEncryption(e));
+    :- Need(IsEncryptedV(outer, virtualFields, newBeacon.loc), E("StandardBeacon " + beacons[0].name + " not defined on an encrypted field."));
+    output := AddStandardBeacons(beacons[1..], outer, key, client, virtualFields, converted[beacons[0].name := I.Standard(newBeacon)]);
+  }
+
+/*
+C.CompoundBeacon
+  nameonly name: string ,
+  nameonly split: Char ,
+  nameonly sensitive: SensitivePartsList ,
+  nameonly nonSensitive: Option<NonSensitivePartsList> ,
+  nameonly constructors: Option<ConstructorList>
+C.SensitivePart
+  nameonly name: string ,
+  nameonly length: BitLength ,
+  nameonly loc: Option<TerminalLocation>
+C.Constructor
+  parts: ConstructorPartList
+C.ConstructorPart
+  nameonly name: string ,
+  nameonly required: bool
+
+I.CompoundBeacon
+  base : BeaconBase,
+  split : char,
+  parts : seq<BeaconPart>, // Non-Sensitive followed by Sensitive
+  construct : ConstructorList
+I.BeaconPart
+  fieldName : FieldName,
+  loc : TerminalLocation,
+  prefix : Prefix,
+  length : Option<BeaconLength>
+IConstructorPart
+  fieldName : FieldName,
+  required : bool
+*/
+
+  function method AddNonSensitiveParts(parts : seq<C.NonSensitivePart>, converted : seq<CB.BeaconPart> := [])
+    : (ret : Result<seq<CB.BeaconPart>, Error>)
+
+  function method AddSensitiveParts(parts : seq<C.SensitivePart>, converted : seq<CB.BeaconPart>)
+    : (ret : Result<seq<CB.BeaconPart>, Error>)
+    ensures ret.Success? ==> 0 < |ret.value|
+
+  function method MakeDefaultConstructor(parts : seq<CB.BeaconPart>, converted : seq<CB.ConstructorPart> := [])
+    : Result<seq<CB.Constructor>, Error>
+    requires 0 < |parts| + |converted|
+  {
+    if |parts| == 0 then
+      Success([CB.Constructor(converted)])
+    else
+      Failure(E(""))
+  }
+
+  function method AddConstructors2(constructors : seq<C.Constructor>, parts : seq<CB.BeaconPart>, converted : seq<CB.Constructor> := [])
+    : Result<seq<CB.Constructor>, Error>
+  {
+    if |constructors| == 0 then
+      Success(converted)
+    else
+      Failure(E(""))
+  }
+  function method AddConstructors(constructors : Option<C.ConstructorList>, parts : seq<CB.BeaconPart>)
+    : (ret : Result<seq<CB.Constructor>, Error>)
+    requires 0 < |parts|
+    requires constructors.Some? ==> 0 < |constructors.value|
+    ensures ret.Success? ==>
+      && (constructors.None? ==> |ret.value| == 1)
+      && (constructors.Some? ==> |ret.value| == |constructors.value|)
+  {
+    if constructors.None? then
+      MakeDefaultConstructor(parts)
+    else
+      AddConstructors2(constructors.value, parts)
+  }
+
+  method {:tailrecursion} AddCompoundBeacons(
+      beacons : seq<C.CompoundBeacon>,
+      outer : DynamoDbItemEncryptorConfig,
+      key : U.Bytes,
+      client: Primitives.AtomicPrimitivesClient,
+      virtualFields : I.VirtualFieldMap,
+      converted : I.BeaconMap := map[])
+    returns (output : Result<I.BeaconMap, Error>)
+    modifies client.Modifies
+    requires client.ValidState()
+    ensures client.ValidState()
+  {
+    if |beacons| == 0 {
+      return Success(converted);
+    }
+    :- Need(beacons[0].name !in converted, E("Duplicate CompoundBeacon name : " + beacons[0].name));
+    var _ :- CheckExists(outer, beacons[0].name, "CompoundBeacon");
+    var newKey :- GetBeaconKey(client, key, beacons[0].name);
+
+    var parts :- AddNonSensitiveParts(beacons[0].nonSensitive.UnwrapOr([]));
+    parts :- AddSensitiveParts(beacons[0].sensitive, parts);
+    :- Need(beacons[0].constructors.None? || 0 < |beacons[0].constructors.value|, E("For beacon " + beacons[0].name + " an empty constructor list was supplied."));
+    var constructors :- AddConstructors(beacons[0].constructors, parts);
+    var newBeacon := CB.CompoundBeacon(
+      B.BeaconBase (
+        client := client,
+        name := beacons[0].name,
+        key := key
+      ),
+      beacons[0].split[0],
+      parts,
+      constructors
+    );
+    output := AddCompoundBeacons(beacons[1..], outer, key, client, virtualFields, converted[beacons[0].name := I.Compound(newBeacon)]);
+  }
+
+  method ConvertBeacons(
+    outer : DynamoDbItemEncryptorConfig,
+    key : U.Bytes,
+    client: Primitives.AtomicPrimitivesClient,
+    virtualFields : I.VirtualFieldMap,
+    standard : seq<C.StandardBeacon>,
+    compound : seq<C.CompoundBeacon>)
+    returns (output : Result<I.BeaconMap, Error>)
+    modifies client.Modifies
+    requires client.ValidState()
+    ensures client.ValidState()
+  {
+    var std :- AddStandardBeacons(standard, outer, key, client, virtualFields);
+    output := AddCompoundBeacons(compound, outer, key, client, virtualFields, std);
+  }
+}
